iris/KernelDecode12.v
@@ -373,6 +373,11 @@ Lemma kd_5ca000ef s : register_lookup misa (sregs s) = MISA_C -> cfg_ok s ->
   = Some (JAL (mword_of_int 1482 : mword 21, Regidx (mword_of_int 1)), s).
 Proof. decode_bridge_ms. Qed.
 
+Lemma kd_6be50513 s : register_lookup misa (sregs s) = MISA_C -> cfg_ok s ->
+  exec (ext_decode (mword_of_int 0x6be50513 : mword 32) : M instruction) s
+  = Some (ITYPE (mword_of_int 1726 : mword 12, Regidx (mword_of_int 10), Regidx (mword_of_int 10), ADDI), s).
+Proof. decode_bridge_ms. Qed.
+
 Lemma kd_777000ef s : register_lookup misa (sregs s) = MISA_C -> cfg_ok s ->
   exec (ext_decode (mword_of_int 0x777000ef : mword 32) : M instruction) s
   = Some (JAL (mword_of_int 3958 : mword 21, Regidx (mword_of_int 1)), s).
